fixing some warnings

ulib/experimental/FStar.Reflection.Typing.fsti
@@ -616,7 +616,7 @@ and comp_ctxt =
   | Ctxt_total  : term_ctxt -> comp_ctxt
   | Ctxt_gtotal : term_ctxt -> comp_ctxt
 
-let rec apply_term_ctxt (e:term_ctxt) (t:term) : term =
+let rec apply_term_ctxt (e:term_ctxt) (t:term) : Tot term (decreases e) =
   match e with
   | Ctxt_hole -> t
   | Ctxt_app_head e arg -> pack_ln (Tv_App (apply_term_ctxt e t) arg)
@@ -636,15 +636,15 @@ let rec apply_term_ctxt (e:term_ctxt) (t:term) : term =
   | Ctxt_match_scrutinee sc ret brs ->
     pack_ln (Tv_Match (apply_term_ctxt sc t) ret brs)
 
-and apply_bv_ctxt (b:bv_ctxt) (t:term) : bv =
+and apply_bv_ctxt (b:bv_ctxt) (t:term) : Tot bv (decreases b) =
   let Ctxt_bv bv_ppname bv_index ty = b in
   pack_bv {bv_ppname; bv_index; bv_sort=apply_term_ctxt ty t}
 
-and apply_binder_ctxt (b:binder_ctxt) (t:term) : binder =
+and apply_binder_ctxt (b:binder_ctxt) (t:term) : Tot binder (decreases b) =
   let Ctxt_binder bv binder_qual binder_attrs = b in
   pack_binder {binder_bv=apply_bv_ctxt bv t; binder_qual; binder_attrs}
 
-and apply_comp_ctxt (c:comp_ctxt) (t:term) : comp =
+and apply_comp_ctxt (c:comp_ctxt) (t:term) : Tot comp (decreases c) =
   match c with
   | Ctxt_total e -> pack_comp (C_Total (apply_term_ctxt e t))
   | Ctxt_gtotal e -> pack_comp (C_GTotal (apply_term_ctxt e t))
@@ -945,7 +945,7 @@ let simplify_umax (#g:R.env) (#t:R.term) (#u:R.universe)
 #push-options "--ifuel 2"
 
 let rec ln' (e:term) (n:int)
-  : bool
+  : Tot bool (decreases e)
   = match inspect_ln e with
     | Tv_UInst _ _
     | Tv_FVar _
